merge ll_mix into ll_fragments
separation into cut-independant and cut-dependant statements is now useless

yalla/ll_fragments.v
@@ -6,14 +6,15 @@
 
 (** * Definitions of various Linear Logic fragments *)
 
-Require Import List.
-
+Require Import Bool_more.
+Require Import List_more.
+Require Import List_Type_more.
 Require Import Permutation_Type_more.
+Require Import Permutation_Type_solve.
 Require Import genperm_Type.
 
 Require Export ll_prop.
 Require Import subs.
-Require Import ll_mix.
 
 
 (** ** Standard linear logic: [ll_ll] (no mix, no axiom, commutative) *)
@@ -52,6 +53,9 @@ Definition pfrag_mix0 := mk_pfrag false NoAxioms true false true.
 
 Definition ll_mix0 := ll pfrag_mix0.
 
+Definition mix0add_pfrag P :=
+  mk_pfrag (pcut P) (pgax P) true (pmix2 P) (pperm P).
+
 Lemma cut_mix0_r : forall A l1 l2, 
   ll_mix0 (dual A :: l1) -> ll_mix0 (A :: l2) -> ll_mix0 (l2 ++ l1).
 Proof with myeeasy.
@@ -71,6 +75,389 @@ induction pi ; try (now econstructor).
 Qed.
 
 (** Provability in [ll_mix0] is equivalent to adding [wn one] in [ll] *)
+
+Lemma mix0_to_ll {P} : pperm P = true -> forall b0 bp l,
+  ll (mk_pfrag P.(pcut) P.(pgax) b0 P.(pmix2) bp) l -> ll P (wn one :: l).
+Proof with myeeasy ; try PCperm_Type_solve.
+intros fp b0 bp l pi.
+eapply (ext_wn_param _ P fp _ (one :: nil)) in pi.
+- eapply ex_r...
+- intros Hcut...
+- simpl ; intros a.
+  eapply ex_r ; [ | apply PCperm_Type_last ].
+  apply wk_r.
+  apply gax_r.
+- intros.
+  eapply de_r.
+  eapply one_r.
+- intros Hpmix2 Hpmix2'.
+  exfalso.
+  simpl in Hpmix2.
+  rewrite Hpmix2 in Hpmix2'.
+  inversion Hpmix2'.
+Qed.
+
+Lemma ll_to_mix0_axat {P} : (forall a, Forall atomic (projT2 (pgax P) a)) ->
+  pperm P = true -> forall l,
+  ll P (wn one :: l) -> ll (mix0add_pfrag P) l.
+Proof with myeeasy ; try PCperm_Type_solve.
+intros Hgax Hperm.
+enough (forall l, ll P l -> forall l' (l0 l1 : list unit),
+  Permutation_Type l (l' ++ map (fun _ => one) l1
+                         ++ map (fun _ => wn one) l0)  ->
+  ll (mix0add_pfrag P) l').
+{ intros l pi.
+  eapply (X _ pi l (tt :: nil) nil)... }
+intros l pi.
+induction pi ; intros l' l0' l1' HP.
+- assert (HP' := HP).
+  symmetry in HP'.
+  apply Permutation_Type_vs_cons_inv in HP'.
+  destruct HP' as [[l'l l'r] Heq] ; simpl in Heq.
+  rewrite Heq in HP.
+  apply Permutation_Type_cons_app_inv in HP.
+  apply Permutation_Type_length_1_inv in HP.
+  apply app_eq_unit_Type in HP.
+  destruct HP as [[Heq1 Heq2] | [Heq1 Heq2]] ; subst ; destruct l' ; inversion Heq ; subst.
+  + destruct l1' ; inversion H0.
+    destruct l0' ; inversion H1.
+  + destruct l' ; inversion H1.
+    * destruct l1' ; inversion H0.
+      destruct l0' ; inversion H2.
+    * destruct l' ; inversion H2.
+      rewrite H3.
+      apply ax_r.
+  + destruct l1' ; inversion H0.
+    destruct l0' ; inversion H1.
+  + destruct l' ; inversion H1.
+    * destruct l1' ; inversion H0.
+      destruct l0' ; inversion H2.
+    * destruct l' ; inversion H2.
+      rewrite H3.
+      eapply ex_r ; [ apply ax_r | ]...
+- rewrite Hperm in p ; simpl in p.
+  eapply IHpi.
+  etransitivity...
+- apply (Permutation_Type_map wn) in p.
+  eapply IHpi.
+  etransitivity...
+- apply Permutation_Type_nil in HP.
+  destruct l' ; inversion HP.
+  rewrite H0.
+  apply mix0_r...
+- apply Permutation_Type_app_app_inv in HP.
+  destruct HP as [[[l1a l2a] [l3a l4a]] [[HP1 HP2] [HP3 HP4]]] ;
+    simpl in HP1 ; simpl in HP2 ; simpl in HP3 ; simpl in HP4.
+  apply Permutation_Type_app_app_inv in HP4.
+  destruct HP4 as [[[l1b l2b] [l3b l4b]] [[HP1b HP2b] [HP3b HP4b]]] ;
+    simpl in HP1b ; simpl in HP2b ; simpl in HP3b ; simpl in HP4b.
+  symmetry in HP1b.
+  apply Permutation_Type_map_inv in HP1b.
+  destruct HP1b as [la Heqa _].
+  decomp_map_Type Heqa ; simpl in Heqa1 ; simpl in Heqa2 ; subst.
+  symmetry in HP2b.
+  apply Permutation_Type_map_inv in HP2b.
+  destruct HP2b as [lb Heqb _].
+  decomp_map_Type Heqb ; simpl in Heqb1 ; simpl in Heqb2 ; subst.
+  apply (Permutation_Type_app_head l2a) in HP4b.
+  assert (IHP1 := Permutation_Type_trans HP2 HP4b).
+  apply (Permutation_Type_app_head l1a) in HP3b.
+  assert (IHP2 := Permutation_Type_trans HP1 HP3b).
+  apply IHpi1 in IHP1.
+  apply IHpi2 in IHP2.
+  symmetry in HP3.
+  eapply ex_r ; [ apply mix2_r | simpl ; rewrite Hperm ; apply HP3 ]...
+- apply Permutation_Type_length_1_inv in HP.
+  destruct l' ; inversion HP.
+  + apply mix0_r...
+  + apply app_eq_nil in H1 ; destruct H1 ; subst.
+    apply one_r.
+- assert (HP' := HP).
+  symmetry in HP'.
+  apply Permutation_Type_vs_cons_inv in HP'.
+  destruct HP' as [[l'l l'r] Heq] ; simpl in Heq.
+  rewrite Heq in HP.
+  apply Permutation_Type_cons_app_inv in HP.
+  dichot_Type_elt_app_exec Heq ; subst.
+  + rewrite app_assoc in HP.
+    apply IHpi in HP.
+    eapply ex_r ; [ apply bot_r | simpl ; rewrite Hperm ]...
+  + dichot_Type_elt_app_exec Heq1 ; subst.
+    * decomp_map_Type Heq0.
+      inversion Heq0.
+    * decomp_map_Type Heq2.
+      inversion Heq2.
+- assert (HP' := HP).
+  symmetry in HP'.
+  apply Permutation_Type_vs_cons_inv in HP'.
+  destruct HP' as [[l'l l'r] Heq] ; simpl in Heq.
+  rewrite Heq in HP.
+  apply Permutation_Type_cons_app_inv in HP.
+  dichot_Type_elt_app_exec Heq ; subst.
+  + rewrite app_assoc in HP.
+    remember (l'l ++ l) as l'.
+    apply Permutation_Type_app_app_inv in HP.
+    destruct HP as [[[l1a l2a] [l3a l4a]] [[HP1 HP2] [HP3 HP4]]] ;
+      simpl in HP1 ; simpl in HP2 ; simpl in HP3 ; simpl in HP4.
+    apply Permutation_Type_app_app_inv in HP4.
+    destruct HP4 as [[[l1b l2b] [l3b l4b]] [[HP1b HP2b] [HP3b HP4b]]] ;
+      simpl in HP1b ; simpl in HP2b ; simpl in HP3b ; simpl in HP4b.
+    symmetry in HP1b.
+    apply Permutation_Type_map_inv in HP1b.
+    destruct HP1b as [la Heqa _].
+    decomp_map_Type Heqa ; simpl in Heqa1 ; simpl in Heqa2 ; subst.
+    symmetry in HP2b.
+    apply Permutation_Type_map_inv in HP2b.
+    destruct HP2b as [lb Heqb _].
+    decomp_map_Type Heqb ; simpl in Heqb1 ; simpl in Heqb2 ; subst.
+    apply (Permutation_Type_app_head l2a) in HP4b.
+    assert (IHP1 := Permutation_Type_trans HP2 HP4b).
+    apply (@Permutation_Type_cons _ A _ eq_refl) in IHP1.
+    rewrite app_comm_cons in IHP1.
+    apply (Permutation_Type_app_head l1a) in HP3b.
+    assert (IHP2 := Permutation_Type_trans HP1 HP3b).
+    apply (@Permutation_Type_cons _ B _ eq_refl) in IHP2.
+    rewrite app_comm_cons in IHP2.
+    apply IHpi1 in IHP1.
+    apply IHpi2 in IHP2.
+    symmetry in HP3.
+    apply (Permutation_Type_cons_app _ _ (tens A B)) in HP3.
+    eapply ex_r ; [ apply tens_r | simpl ; rewrite Hperm ; apply HP3 ]...
+  + dichot_Type_elt_app_exec Heq1 ; subst.
+    * exfalso.
+      decomp_map_Type Heq0 ; inversion Heq0.
+    * decomp_map_Type Heq2.
+      inversion Heq2.
+- assert (HP' := HP).
+  symmetry in HP'.
+  apply Permutation_Type_vs_cons_inv in HP'.
+  destruct HP' as [[l'l l'r] Heq] ; simpl in Heq.
+  rewrite Heq in HP.
+  apply Permutation_Type_cons_app_inv in HP.
+  dichot_Type_elt_app_exec Heq ; subst.
+  + rewrite app_assoc in HP.
+    apply (@Permutation_Type_cons _ B _ eq_refl) in HP.
+    apply (@Permutation_Type_cons _ A _ eq_refl) in HP.
+    rewrite 2 app_comm_cons in HP.
+    apply IHpi in HP.
+    eapply ex_r ; [ apply parr_r | simpl ; rewrite Hperm ]...
+  + dichot_Type_elt_app_exec Heq1 ; subst.
+    * decomp_map_Type Heq0.
+      inversion Heq0.
+    * decomp_map_Type Heq2.
+      inversion Heq2.
+- assert (HP' := HP).
+  symmetry in HP'.
+  apply Permutation_Type_vs_cons_inv in HP'.
+  destruct HP' as [[l'l l'r] Heq] ; simpl in Heq.
+  rewrite Heq in HP.
+  apply Permutation_Type_cons_app_inv in HP.
+  dichot_Type_elt_app_exec Heq ; subst.
+  + eapply ex_r ; [ apply top_r
+                  | simpl ; rewrite Hperm ; apply Permutation_Type_middle ]...
+  + dichot_Type_elt_app_exec Heq1 ; subst.
+    * decomp_map_Type Heq0.
+      inversion Heq0.
+    * decomp_map_Type Heq2.
+      inversion Heq2.
+- assert (HP' := HP).
+  symmetry in HP'.
+  apply Permutation_Type_vs_cons_inv in HP'.
+  destruct HP' as [[l'l l'r] Heq] ; simpl in Heq.
+  rewrite Heq in HP.
+  apply Permutation_Type_cons_app_inv in HP.
+  dichot_Type_elt_app_exec Heq ; subst.
+  + rewrite app_assoc in HP.
+    apply (@Permutation_Type_cons _ A _ eq_refl) in HP.
+    rewrite app_comm_cons in HP.
+    apply IHpi in HP.
+    eapply ex_r ; [ apply plus_r1 | simpl ; rewrite Hperm ]...
+  + dichot_Type_elt_app_exec Heq1 ; subst.
+    * decomp_map_Type Heq0.
+      inversion Heq0.
+    * decomp_map_Type Heq2.
+      inversion Heq2.
+- assert (HP' := HP).
+  symmetry in HP'.
+  apply Permutation_Type_vs_cons_inv in HP'.
+  destruct HP' as [[l'l l'r] Heq] ; simpl in Heq.
+  rewrite Heq in HP.
+  apply Permutation_Type_cons_app_inv in HP.
+  dichot_Type_elt_app_exec Heq ; subst.
+  + rewrite app_assoc in HP.
+    apply (@Permutation_Type_cons _ A _ eq_refl) in HP.
+    rewrite app_comm_cons in HP.
+    apply IHpi in HP.
+    eapply ex_r ; [ apply plus_r2 | simpl ; rewrite Hperm ]...
+  + dichot_Type_elt_app_exec Heq1 ; subst.
+    * decomp_map_Type Heq0.
+      inversion Heq0.
+    * decomp_map_Type Heq2.
+      inversion Heq2.
+- assert (HP' := HP).
+  symmetry in HP'.
+  apply Permutation_Type_vs_cons_inv in HP'.
+  destruct HP' as [[l'l l'r] Heq] ; simpl in Heq.
+  rewrite Heq in HP.
+  apply Permutation_Type_cons_app_inv in HP.
+  dichot_Type_elt_app_exec Heq ; subst.
+  + rewrite app_assoc in HP.
+    assert (HP2 := HP).
+    apply (@Permutation_Type_cons _ A _ eq_refl) in HP.
+    rewrite app_comm_cons in HP.
+    apply IHpi1 in HP.
+    apply (@Permutation_Type_cons _ B _ eq_refl) in HP2.
+    rewrite app_comm_cons in HP2.
+    apply IHpi2 in HP2.
+    eapply ex_r ; [ apply with_r
+                  | simpl ; rewrite Hperm ; apply Permutation_Type_middle ]...
+  + dichot_Type_elt_app_exec Heq1 ; subst.
+    * decomp_map_Type Heq0.
+      inversion Heq0.
+    * decomp_map_Type Heq2.
+      inversion Heq2.
+- assert (HP' := HP).
+  symmetry in HP'.
+  apply Permutation_Type_vs_cons_inv in HP'.
+  destruct HP' as [[l'l l'r] Heq] ; simpl in Heq.
+  rewrite Heq in HP.
+  apply Permutation_Type_cons_app_inv in HP.
+  dichot_Type_elt_app_exec Heq ; subst.
+  + symmetry in HP.
+    apply Permutation_Type_map_inv in HP.
+    destruct HP as [l' Heq HP].
+    decomp_map_Type Heq ;
+      simpl in Heq1 ; simpl in Heq2 ; simpl in Heq3 ; simpl in Heq5 ; subst ;
+      simpl in HP.
+    apply (Permutation_Type_map wn) in HP.
+    list_simpl in HP.
+    rewrite app_assoc in HP.
+    rewrite <- map_app in HP.
+    apply (@Permutation_Type_cons _ A _ eq_refl) in HP.
+    rewrite app_comm_cons in HP.
+    rewrite <- Heq2 in HP.
+    rewrite <- Heq5 in HP.
+    apply IHpi in HP.
+    eapply ex_r ; [ apply oc_r | simpl ; rewrite Hperm ]...
+  + dichot_Type_elt_app_exec Heq1 ; subst.
+    * decomp_map_Type Heq0.
+      inversion Heq0.
+    * decomp_map_Type Heq2.
+      inversion Heq2.
+- assert (HP' := HP).
+  symmetry in HP'.
+  apply Permutation_Type_vs_cons_inv in HP'.
+  destruct HP' as [[l'l l'r] Heq] ; simpl in Heq.
+  rewrite Heq in HP.
+  apply Permutation_Type_cons_app_inv in HP.
+  dichot_Type_elt_app_exec Heq ; subst.
+  + rewrite app_assoc in HP.
+    apply (@Permutation_Type_cons _ A _ eq_refl) in HP.
+    rewrite app_comm_cons in HP.
+    apply IHpi in HP.
+    eapply ex_r ; [ apply de_r | simpl ; rewrite Hperm ]...
+  + dichot_Type_elt_app_exec Heq1 ; subst.
+    * decomp_map_Type Heq0.
+      inversion Heq0.
+    * decomp_map_Type Heq2 ; simpl in Heq1 ; simpl in Heq2 ; simpl in Heq3 ; subst ; simpl in HP.
+      inversion Heq2 ; subst.
+      list_simpl in HP ; rewrite <- map_app in HP.
+      apply (@Permutation_Type_cons _ one _ eq_refl) in HP.
+      assert (Permutation_Type (one :: l)
+                               (l' ++ map (fun _ : unit => one) (tt :: l1')
+                                   ++ map (fun _ : unit => wn one) (l1 ++ l4)))
+        as HP' by (etransitivity ; [ apply HP | ] ; perm_Type_solve). 
+      apply IHpi in HP'...
+- assert (HP' := HP).
+  symmetry in HP'.
+  apply Permutation_Type_vs_cons_inv in HP'.
+  destruct HP' as [[l'l l'r] Heq] ; simpl in Heq.
+  rewrite Heq in HP.
+  apply Permutation_Type_cons_app_inv in HP.
+  dichot_Type_elt_app_exec Heq ; subst.
+  + rewrite app_assoc in HP.
+    apply IHpi in HP.
+    eapply ex_r ; [ apply wk_r | simpl ; rewrite Hperm ]...
+  + dichot_Type_elt_app_exec Heq1 ; subst.
+    * decomp_map_Type Heq0.
+      inversion Heq0.
+    * decomp_map_Type Heq2 ; simpl in Heq1 ; simpl in Heq2 ; simpl in Heq3 ; subst ; simpl in HP.
+      inversion Heq2 ; subst.
+      list_simpl in HP ; rewrite <- map_app in HP.
+      apply IHpi in HP...
+- assert (HP' := HP).
+  symmetry in HP'.
+  apply Permutation_Type_vs_cons_inv in HP'.
+  destruct HP' as [[l'l l'r] Heq] ; simpl in Heq.
+  rewrite Heq in HP.
+  apply Permutation_Type_cons_app_inv in HP.
+  dichot_Type_elt_app_exec Heq ; subst.
+  + rewrite app_assoc in HP.
+    apply (@Permutation_Type_cons _ (wn A) _ eq_refl) in HP.
+    apply (@Permutation_Type_cons _ (wn A) _ eq_refl) in HP.
+    rewrite 2 app_comm_cons in HP.
+    apply IHpi in HP.
+    eapply ex_r ; [ apply co_r | simpl ; rewrite Hperm ]...
+  + dichot_Type_elt_app_exec Heq1 ; subst.
+    * decomp_map_Type Heq0.
+      inversion Heq0.
+    * decomp_map_Type Heq2 ; simpl in Heq1 ; simpl in Heq2 ; simpl in Heq3 ; subst ; simpl in HP.
+      inversion Heq2 ; subst.
+      list_simpl in HP ; rewrite <- map_app in HP.
+      apply (@Permutation_Type_cons _ (wn one) _ eq_refl) in HP.
+      apply (@Permutation_Type_cons _ (wn one) _ eq_refl) in HP.
+      assert (Permutation_Type (wn one :: wn one :: l)
+                               (l' ++ map (fun _ : unit => one) l1' ++
+                                  map (fun _ : unit => wn one) (tt :: tt :: l1 ++ l4)))
+        as HP' by (etransitivity ; [ apply HP | perm_Type_solve ]).
+      apply IHpi in HP'...
+- apply Permutation_Type_app_app_inv in HP.
+  destruct HP as [[[l1a l2a] [l3a l4a]] [[HP1 HP2] [HP3 HP4]]] ;
+    simpl in HP1 ; simpl in HP2 ; simpl in HP3 ; simpl in HP4.
+  apply Permutation_Type_app_app_inv in HP4.
+  destruct HP4 as [[[l1b l2b] [l3b l4b]] [[HP1b HP2b] [HP3b HP4b]]] ;
+    simpl in HP1b ; simpl in HP2b ; simpl in HP3b ; simpl in HP4b.
+  symmetry in HP1b.
+  apply Permutation_Type_map_inv in HP1b.
+  destruct HP1b as [la Heqa _].
+  decomp_map_Type Heqa ; simpl in Heqa1 ; simpl in Heqa2 ; subst.
+  symmetry in HP2b.
+  apply Permutation_Type_map_inv in HP2b.
+  destruct HP2b as [lb Heqb _].
+  decomp_map_Type Heqb ; simpl in Heqb1 ; simpl in Heqb2 ; subst.
+  apply (Permutation_Type_app_head l2a) in HP4b.
+  assert (IHP1 := Permutation_Type_trans HP2 HP4b).
+  apply (@Permutation_Type_cons _ (dual A) _ eq_refl) in IHP1.
+  rewrite app_comm_cons in IHP1.
+  apply (Permutation_Type_app_head l1a) in HP3b.
+  assert (IHP2 := Permutation_Type_trans HP1 HP3b).
+  apply (@Permutation_Type_cons _ A _ eq_refl) in IHP2.
+  rewrite app_comm_cons in IHP2.
+  apply IHpi1 in IHP1.
+  apply IHpi2 in IHP2.
+  symmetry in HP3.
+  eapply ex_r ; [ eapply cut_r | simpl ; rewrite Hperm ; apply HP3 ]...
+- destruct l1' ; destruct l0' ; simpl in HP.
+  + eapply ex_r ; [ apply gax_r | simpl ; rewrite Hperm ]...
+  + exfalso.
+    apply Permutation_Type_vs_elt_inv in HP.
+    specialize (Hgax a).
+    destruct HP as [[l1 l2] Heq] ; rewrite Heq in Hgax.
+    apply Forall_elt in Hgax.
+    inversion Hgax.
+  + exfalso.
+    apply Permutation_Type_vs_elt_inv in HP.
+    specialize (Hgax a).
+    destruct HP as [[l1 l2] Heq] ; rewrite Heq in Hgax.
+    apply Forall_elt in Hgax.
+    inversion Hgax.
+  + exfalso.
+    apply Permutation_Type_vs_elt_inv in HP.
+    specialize (Hgax a).
+    destruct HP as [[l1 l2] Heq] ; rewrite Heq in Hgax.
+    apply Forall_elt in Hgax.
+    inversion Hgax.
+Qed.
 
 Lemma ll_to_mix0_cut {P} : forall l,
   ll P (wn one :: l) -> ll (mk_pfrag true P.(pgax) true P.(pmix2) P.(pperm)) l.
@@ -207,6 +594,9 @@ Definition pfrag_mix2 := mk_pfrag false NoAxioms false true true.
 
 Definition ll_mix2 := ll pfrag_mix2.
 
+Definition mix2add_pfrag P :=
+  mk_pfrag (pcut P) (pgax P) (pmix0 P) true (pperm P).
+
 Lemma cut_mix2_r : forall A l1 l2,
   ll_mix2 (dual A :: l1) -> ll_mix2 (A :: l2) -> ll_mix2 (l2 ++ l1).
 Proof with myeeasy.
@@ -226,6 +616,430 @@ induction pi ; try (now econstructor).
 Qed.
 
 (** Provability in [ll_mix2] is equivalent to adding [wn (tens bot bot)] in [ll] *)
+
+Lemma mix2_to_ll {P} : pperm P = true -> forall b2 bp l,
+  ll (mk_pfrag P.(pcut) P.(pgax) P.(pmix0) b2 bp) l -> ll P (wn (tens bot bot) :: l).
+Proof with myeeasy ; try PCperm_Type_solve.
+intros fp b2 bp l pi.
+eapply (ext_wn_param _ P fp _ (tens bot bot :: nil)) in pi.
+- eapply ex_r...
+- intros Hcut...
+- simpl ; intros a.
+  eapply ex_r ; [ | apply PCperm_Type_last ].
+  apply wk_r.
+  apply gax_r.
+- intros Hpmix0 Hpmix0'.
+  exfalso.
+  simpl in Hpmix0.
+  rewrite Hpmix0 in Hpmix0'.
+  inversion Hpmix0'.
+- intros _ _ l1 l2 pi1 pi2.
+  apply (ex_r _ (wn (tens bot bot) :: l2 ++ l1))...
+  apply co_r.
+  apply co_r.
+  apply de_r.
+  eapply ex_r.
+  + apply tens_r ; apply bot_r ; [ apply pi1 | apply pi2 ].
+  + rewrite fp...
+Qed.
+
+Lemma ll_to_mix2_axat {P} : (forall a, Forall atomic (projT2 (pgax P) a)) ->
+  pperm P = true -> forall l,
+  ll P (wn (tens bot bot) :: l) -> ll (mix2add_pfrag P) l.
+Proof with myeeasy ; try PCperm_Type_solve.
+intros Hgax Hperm.
+enough (forall l, ll P l -> forall l' (l0 l1 : list unit),
+  Permutation_Type l (l' ++ map (fun _ => tens bot bot) l1
+                         ++ map (fun _ => wn (tens bot bot)) l0)  ->
+  ll (mix2add_pfrag P) l').
+{ intros l pi.
+  eapply (X _ pi l (tt :: nil) nil)... }
+intros l pi.
+induction pi ; intros l' l0' l1' HP.
+- assert (HP' := HP).
+  symmetry in HP'.
+  apply Permutation_Type_vs_cons_inv in HP'.
+  destruct HP' as [[l'l l'r] Heq] ; simpl in Heq.
+  rewrite Heq in HP.
+  apply Permutation_Type_cons_app_inv in HP.
+  apply Permutation_Type_length_1_inv in HP.
+  apply app_eq_unit_Type in HP.
+  destruct HP as [[Heq1 Heq2] | [Heq1 Heq2]] ; subst ; destruct l' ; inversion Heq ; subst.
+  + destruct l1' ; inversion H0.
+    destruct l0' ; inversion H1.
+  + destruct l' ; inversion H1.
+    * destruct l1' ; inversion H0.
+      destruct l0' ; inversion H2.
+    * destruct l' ; inversion H2.
+      rewrite H3.
+      apply ax_r.
+  + destruct l1' ; inversion H0.
+    destruct l0' ; inversion H1.
+  + destruct l' ; inversion H1.
+    * destruct l1' ; inversion H0.
+      destruct l0' ; inversion H2.
+    * destruct l' ; inversion H2.
+      rewrite H3.
+      eapply ex_r ; [ apply ax_r | ]...
+- rewrite Hperm in p ; simpl in p.
+  eapply IHpi.
+  etransitivity...
+- apply (Permutation_Type_map wn) in p.
+  eapply IHpi.
+  etransitivity...
+- apply Permutation_Type_nil in HP.
+  destruct l' ; inversion HP.
+  rewrite H0.
+  apply mix0_r...
+- apply Permutation_Type_app_app_inv in HP.
+  destruct HP as [[[l1a l2a] [l3a l4a]] [[HP1 HP2] [HP3 HP4]]] ;
+    simpl in HP1 ; simpl in HP2 ; simpl in HP3 ; simpl in HP4.
+  apply Permutation_Type_app_app_inv in HP4.
+  destruct HP4 as [[[l1b l2b] [l3b l4b]] [[HP1b HP2b] [HP3b HP4b]]] ;
+    simpl in HP1b ; simpl in HP2b ; simpl in HP3b ; simpl in HP4b.
+  symmetry in HP1b.
+  apply Permutation_Type_map_inv in HP1b.
+  destruct HP1b as [la Heqa _].
+  decomp_map_Type Heqa ; simpl in Heqa1 ; simpl in Heqa2 ; subst.
+  symmetry in HP2b.
+  apply Permutation_Type_map_inv in HP2b.
+  destruct HP2b as [lb Heqb _].
+  decomp_map_Type Heqb ; simpl in Heqb1 ; simpl in Heqb2 ; subst.
+  apply (Permutation_Type_app_head l2a) in HP4b.
+  assert (IHP1 := Permutation_Type_trans HP2 HP4b).
+  apply (Permutation_Type_app_head l1a) in HP3b.
+  assert (IHP2 := Permutation_Type_trans HP1 HP3b).
+  apply IHpi1 in IHP1.
+  apply IHpi2 in IHP2.
+  symmetry in HP3.
+  eapply ex_r ; [ apply mix2_r | simpl ; rewrite Hperm ; apply HP3 ]...
+- apply Permutation_Type_length_1_inv in HP.
+  destruct l' ; inversion HP.
+  + destruct l1' ; inversion H0.
+    destruct l0' ; inversion H1.
+  + apply app_eq_nil in H1 ; destruct H1 ; subst.
+    apply one_r.
+- assert (HP' := HP).
+  symmetry in HP'.
+  apply Permutation_Type_vs_cons_inv in HP'.
+  destruct HP' as [[l'l l'r] Heq] ; simpl in Heq.
+  rewrite Heq in HP.
+  apply Permutation_Type_cons_app_inv in HP.
+  dichot_Type_elt_app_exec Heq ; subst.
+  + rewrite app_assoc in HP.
+    apply IHpi in HP.
+    eapply ex_r ; [ apply bot_r | simpl ; rewrite Hperm ]...
+  + dichot_Type_elt_app_exec Heq1 ; subst.
+    * decomp_map_Type Heq0.
+      inversion Heq0.
+    * decomp_map_Type Heq2.
+      inversion Heq2.
+- assert (HP' := HP).
+  symmetry in HP'.
+  apply Permutation_Type_vs_cons_inv in HP'.
+  destruct HP' as [[l'l l'r] Heq] ; simpl in Heq.
+  rewrite Heq in HP.
+  apply Permutation_Type_cons_app_inv in HP.
+  dichot_Type_elt_app_exec Heq ; subst.
+  + rewrite app_assoc in HP.
+    remember (l'l ++ l) as l'.
+    apply Permutation_Type_app_app_inv in HP.
+    destruct HP as [[[l1a l2a] [l3a l4a]] [[HP1 HP2] [HP3 HP4]]] ;
+      simpl in HP1 ; simpl in HP2 ; simpl in HP3 ; simpl in HP4.
+    apply Permutation_Type_app_app_inv in HP4.
+    destruct HP4 as [[[l1b l2b] [l3b l4b]] [[HP1b HP2b] [HP3b HP4b]]] ;
+      simpl in HP1b ; simpl in HP2b ; simpl in HP3b ; simpl in HP4b.
+    symmetry in HP1b.
+    apply Permutation_Type_map_inv in HP1b.
+    destruct HP1b as [la Heqa _].
+    decomp_map_Type Heqa ; simpl in Heqa1 ; simpl in Heqa2 ; subst.
+    symmetry in HP2b.
+    apply Permutation_Type_map_inv in HP2b.
+    destruct HP2b as [lb Heqb _].
+    decomp_map_Type Heqb ; simpl in Heqb1 ; simpl in Heqb2 ; subst.
+    apply (Permutation_Type_app_head l2a) in HP4b.
+    assert (IHP1 := Permutation_Type_trans HP2 HP4b).
+    apply (@Permutation_Type_cons _ A _ eq_refl) in IHP1.
+    rewrite app_comm_cons in IHP1.
+    apply (Permutation_Type_app_head l1a) in HP3b.
+    assert (IHP2 := Permutation_Type_trans HP1 HP3b).
+    apply (@Permutation_Type_cons _ B _ eq_refl) in IHP2.
+    rewrite app_comm_cons in IHP2.
+    apply IHpi1 in IHP1.
+    apply IHpi2 in IHP2.
+    symmetry in HP3.
+    apply (Permutation_Type_cons_app _ _ (tens A B)) in HP3.
+    eapply ex_r ; [ apply tens_r | simpl ; rewrite Hperm ; apply HP3 ]...
+  + dichot_Type_elt_app_exec Heq1 ; subst.
+    * decomp_map_Type Heq0.
+      inversion Heq0 ; subst ; list_simpl in HP.
+      rewrite (app_assoc (map _ l4)) in HP.
+      rewrite <- map_app in HP.
+      remember (l4 ++ l6) as l0 ; clear Heql0.
+      apply Permutation_Type_app_app_inv in HP.
+      destruct HP as [[[l1a l2a] [l3a l4a]] [[HP1 HP2] [HP3 HP4]]] ;
+        simpl in HP1 ; simpl in HP2 ; simpl in HP3 ; simpl in HP4.
+      apply Permutation_Type_app_app_inv in HP4.
+      destruct HP4 as [[[l1b l2b] [l3b l4b]] [[HP1b HP2b] [HP3b HP4b]]] ;
+        simpl in HP1b ; simpl in HP2b ; simpl in HP3b ; simpl in HP4b.
+      symmetry in HP1b.
+      apply Permutation_Type_map_inv in HP1b.
+      destruct HP1b as [la Heqa _].
+      decomp_map_Type Heqa ; simpl in Heqa1 ; simpl in Heqa2 ; subst.
+      symmetry in HP2b.
+      apply Permutation_Type_map_inv in HP2b.
+      destruct HP2b as [lb Heqb _].
+      decomp_map_Type Heqb ; simpl in Heqb1 ; simpl in Heqb2 ; subst.
+      apply (Permutation_Type_app_head l2a) in HP4b.
+      assert (IHP1 := Permutation_Type_trans HP2 HP4b).
+      apply (@Permutation_Type_cons _ bot _ eq_refl) in IHP1.
+      rewrite app_comm_cons in IHP1.
+      apply IHpi1 in IHP1.
+      rewrite <- app_nil_l in IHP1.
+      eapply bot_rev_axat in IHP1 ; [ | apply Hgax | reflexivity ].
+      list_simpl in IHP1.
+      apply (Permutation_Type_app_head l1a) in HP3b.
+      assert (IHP2 := Permutation_Type_trans HP1 HP3b).
+      apply (@Permutation_Type_cons _ bot _ eq_refl) in IHP2.
+      rewrite app_comm_cons in IHP2.
+      apply IHpi2 in IHP2.
+      rewrite <- app_nil_l in IHP2.
+      eapply bot_rev_axat in IHP2 ; [ | apply Hgax | reflexivity ].
+      list_simpl in IHP2.
+      assert (Permutation_Type (l2a ++ l1a) l') as HP' by perm_Type_solve.
+      eapply ex_r ; [ apply mix2_r | simpl ; rewrite Hperm ; apply HP' ]...
+    * decomp_map_Type Heq2.
+      inversion Heq2.
+- assert (HP' := HP).
+  symmetry in HP'.
+  apply Permutation_Type_vs_cons_inv in HP'.
+  destruct HP' as [[l'l l'r] Heq] ; simpl in Heq.
+  rewrite Heq in HP.
+  apply Permutation_Type_cons_app_inv in HP.
+  dichot_Type_elt_app_exec Heq ; subst.
+  + rewrite app_assoc in HP.
+    apply (@Permutation_Type_cons _ B _ eq_refl) in HP.
+    apply (@Permutation_Type_cons _ A _ eq_refl) in HP.
+    rewrite 2 app_comm_cons in HP.
+    apply IHpi in HP.
+    eapply ex_r ; [ apply parr_r | simpl ; rewrite Hperm ]...
+  + dichot_Type_elt_app_exec Heq1 ; subst.
+    * decomp_map_Type Heq0.
+      inversion Heq0.
+    * decomp_map_Type Heq2.
+      inversion Heq2.
+- assert (HP' := HP).
+  symmetry in HP'.
+  apply Permutation_Type_vs_cons_inv in HP'.
+  destruct HP' as [[l'l l'r] Heq] ; simpl in Heq.
+  rewrite Heq in HP.
+  apply Permutation_Type_cons_app_inv in HP.
+  dichot_Type_elt_app_exec Heq ; subst.
+  + eapply ex_r ; [ apply top_r
+                  | simpl ; rewrite Hperm ; apply Permutation_Type_middle ]...
+  + dichot_Type_elt_app_exec Heq1 ; subst.
+    * decomp_map_Type Heq0.
+      inversion Heq0.
+    * decomp_map_Type Heq2.
+      inversion Heq2.
+- assert (HP' := HP).
+  symmetry in HP'.
+  apply Permutation_Type_vs_cons_inv in HP'.
+  destruct HP' as [[l'l l'r] Heq] ; simpl in Heq.
+  rewrite Heq in HP.
+  apply Permutation_Type_cons_app_inv in HP.
+  dichot_Type_elt_app_exec Heq ; subst.
+  + rewrite app_assoc in HP.
+    apply (@Permutation_Type_cons _ A _ eq_refl) in HP.
+    rewrite app_comm_cons in HP.
+    apply IHpi in HP.
+    eapply ex_r ; [ apply plus_r1 | simpl ; rewrite Hperm ]...
+  + dichot_Type_elt_app_exec Heq1 ; subst.
+    * decomp_map_Type Heq0.
+      inversion Heq0.
+    * decomp_map_Type Heq2.
+      inversion Heq2.
+- assert (HP' := HP).
+  symmetry in HP'.
+  apply Permutation_Type_vs_cons_inv in HP'.
+  destruct HP' as [[l'l l'r] Heq] ; simpl in Heq.
+  rewrite Heq in HP.
+  apply Permutation_Type_cons_app_inv in HP.
+  dichot_Type_elt_app_exec Heq ; subst.
+  + rewrite app_assoc in HP.
+    apply (@Permutation_Type_cons _ A _ eq_refl) in HP.
+    rewrite app_comm_cons in HP.
+    apply IHpi in HP.
+    eapply ex_r ; [ apply plus_r2 | simpl ; rewrite Hperm ]...
+  + dichot_Type_elt_app_exec Heq1 ; subst.
+    * decomp_map_Type Heq0.
+      inversion Heq0.
+    * decomp_map_Type Heq2.
+      inversion Heq2.
+- assert (HP' := HP).
+  symmetry in HP'.
+  apply Permutation_Type_vs_cons_inv in HP'.
+  destruct HP' as [[l'l l'r] Heq] ; simpl in Heq.
+  rewrite Heq in HP.
+  apply Permutation_Type_cons_app_inv in HP.
+  dichot_Type_elt_app_exec Heq ; subst.
+  + rewrite app_assoc in HP.
+    assert (HP2 := HP).
+    apply (@Permutation_Type_cons _ A _ eq_refl) in HP.
+    rewrite app_comm_cons in HP.
+    apply IHpi1 in HP.
+    apply (@Permutation_Type_cons _ B _ eq_refl) in HP2.
+    rewrite app_comm_cons in HP2.
+    apply IHpi2 in HP2.
+    eapply ex_r ; [ apply with_r
+                  | simpl ; rewrite Hperm ; apply Permutation_Type_middle ]...
+  + dichot_Type_elt_app_exec Heq1 ; subst.
+    * decomp_map_Type Heq0.
+      inversion Heq0.
+    * decomp_map_Type Heq2.
+      inversion Heq2.
+- assert (HP' := HP).
+  symmetry in HP'.
+  apply Permutation_Type_vs_cons_inv in HP'.
+  destruct HP' as [[l'l l'r] Heq] ; simpl in Heq.
+  rewrite Heq in HP.
+  apply Permutation_Type_cons_app_inv in HP.
+  dichot_Type_elt_app_exec Heq ; subst.
+  + symmetry in HP.
+    apply Permutation_Type_map_inv in HP.
+    destruct HP as [l' Heq HP].
+    decomp_map_Type Heq ;
+      simpl in Heq1 ; simpl in Heq2 ; simpl in Heq3 ; simpl in Heq5 ; subst ;
+      simpl in HP.
+    apply (Permutation_Type_map wn) in HP.
+    list_simpl in HP.
+    rewrite app_assoc in HP.
+    rewrite <- map_app in HP.
+    apply (@Permutation_Type_cons _ A _ eq_refl) in HP.
+    rewrite app_comm_cons in HP.
+    rewrite <- Heq2 in HP.
+    rewrite <- Heq5 in HP.
+    apply IHpi in HP.
+    eapply ex_r ; [ apply oc_r | simpl ; rewrite Hperm ]...
+  + dichot_Type_elt_app_exec Heq1 ; subst.
+    * decomp_map_Type Heq0.
+      inversion Heq0.
+    * decomp_map_Type Heq2.
+      inversion Heq2.
+- assert (HP' := HP).
+  symmetry in HP'.
+  apply Permutation_Type_vs_cons_inv in HP'.
+  destruct HP' as [[l'l l'r] Heq] ; simpl in Heq.
+  rewrite Heq in HP.
+  apply Permutation_Type_cons_app_inv in HP.
+  dichot_Type_elt_app_exec Heq ; subst.
+  + rewrite app_assoc in HP.
+    apply (@Permutation_Type_cons _ A _ eq_refl) in HP.
+    rewrite app_comm_cons in HP.
+    apply IHpi in HP.
+    eapply ex_r ; [ apply de_r | simpl ; rewrite Hperm ]...
+  + dichot_Type_elt_app_exec Heq1 ; subst.
+    * decomp_map_Type Heq0.
+      inversion Heq0.
+    * decomp_map_Type Heq2 ; simpl in Heq1 ; simpl in Heq2 ; simpl in Heq3 ; subst ; simpl in HP.
+      inversion Heq2 ; subst.
+      list_simpl in HP ; rewrite <- map_app in HP.
+      apply (@Permutation_Type_cons _ (tens bot bot) _ eq_refl) in HP.
+      assert (Permutation_Type (tens bot bot :: l)
+                               (l' ++ map (fun _ : unit => tens bot bot) (tt :: l1')
+                                   ++ map (fun _ : unit => wn (tens bot bot)) (l1 ++ l4)))
+        as HP' by (etransitivity ; [ apply HP | ] ; perm_Type_solve). 
+      apply IHpi in HP'...
+- assert (HP' := HP).
+  symmetry in HP'.
+  apply Permutation_Type_vs_cons_inv in HP'.
+  destruct HP' as [[l'l l'r] Heq] ; simpl in Heq.
+  rewrite Heq in HP.
+  apply Permutation_Type_cons_app_inv in HP.
+  dichot_Type_elt_app_exec Heq ; subst.
+  + rewrite app_assoc in HP.
+    apply IHpi in HP.
+    eapply ex_r ; [ apply wk_r | simpl ; rewrite Hperm ]...
+  + dichot_Type_elt_app_exec Heq1 ; subst.
+    * decomp_map_Type Heq0.
+      inversion Heq0.
+    * decomp_map_Type Heq2 ; simpl in Heq1 ; simpl in Heq2 ; simpl in Heq3 ; subst ; simpl in HP.
+      inversion Heq2 ; subst.
+      list_simpl in HP ; rewrite <- map_app in HP.
+      apply IHpi in HP...
+- assert (HP' := HP).
+  symmetry in HP'.
+  apply Permutation_Type_vs_cons_inv in HP'.
+  destruct HP' as [[l'l l'r] Heq] ; simpl in Heq.
+  rewrite Heq in HP.
+  apply Permutation_Type_cons_app_inv in HP.
+  dichot_Type_elt_app_exec Heq ; subst.
+  + rewrite app_assoc in HP.
+    apply (@Permutation_Type_cons _ (wn A) _ eq_refl) in HP.
+    apply (@Permutation_Type_cons _ (wn A) _ eq_refl) in HP.
+    rewrite 3 app_comm_cons in HP.
+    apply IHpi in HP.
+    eapply ex_r ; [ apply co_r | simpl ; rewrite Hperm ]...
+  + dichot_Type_elt_app_exec Heq1 ; subst.
+    * decomp_map_Type Heq0.
+      inversion Heq0.
+    * decomp_map_Type Heq2 ; simpl in Heq1 ; simpl in Heq2 ; simpl in Heq3 ; subst ; simpl in HP.
+      inversion Heq2 ; subst.
+      list_simpl in HP ; rewrite <- map_app in HP.
+      apply (@Permutation_Type_cons _ (wn (tens bot bot)) _ eq_refl) in HP.
+      apply (@Permutation_Type_cons _ (wn (tens bot bot)) _ eq_refl) in HP.
+      assert (Permutation_Type (wn (tens bot bot) :: wn (tens bot bot) :: l)
+                               (l' ++ map (fun _ : unit => tens bot bot) l1' ++
+                                  map (fun _ : unit => wn (tens bot bot)) (tt :: tt :: l1 ++ l4)))
+        as HP' by (etransitivity ; [ apply HP | perm_Type_solve ]).
+      apply IHpi in HP'...
+- apply Permutation_Type_app_app_inv in HP.
+  destruct HP as [[[l1a l2a] [l3a l4a]] [[HP1 HP2] [HP3 HP4]]] ;
+    simpl in HP1 ; simpl in HP2 ; simpl in HP3 ; simpl in HP4.
+  apply Permutation_Type_app_app_inv in HP4.
+  destruct HP4 as [[[l1b l2b] [l3b l4b]] [[HP1b HP2b] [HP3b HP4b]]] ;
+    simpl in HP1b ; simpl in HP2b ; simpl in HP3b ; simpl in HP4b.
+  symmetry in HP1b.
+  apply Permutation_Type_map_inv in HP1b.
+  destruct HP1b as [la Heqa _].
+  decomp_map_Type Heqa ; simpl in Heqa1 ; simpl in Heqa2 ; subst.
+  symmetry in HP2b.
+  apply Permutation_Type_map_inv in HP2b.
+  destruct HP2b as [lb Heqb _].
+  decomp_map_Type Heqb ; simpl in Heqb1 ; simpl in Heqb2 ; subst.
+  apply (Permutation_Type_app_head l2a) in HP4b.
+  assert (IHP1 := Permutation_Type_trans HP2 HP4b).
+  apply (@Permutation_Type_cons _ (dual A) _ eq_refl) in IHP1.
+  rewrite app_comm_cons in IHP1.
+  apply (Permutation_Type_app_head l1a) in HP3b.
+  assert (IHP2 := Permutation_Type_trans HP1 HP3b).
+  apply (@Permutation_Type_cons _ A _ eq_refl) in IHP2.
+  rewrite app_comm_cons in IHP2.
+  apply IHpi1 in IHP1.
+  apply IHpi2 in IHP2.
+  symmetry in HP3.
+  eapply ex_r ; [ eapply cut_r | simpl ; rewrite Hperm ; apply HP3 ]...
+- destruct l1' ; destruct l0' ; simpl in HP.
+  + eapply ex_r ; [ apply gax_r | simpl ; rewrite Hperm ]...
+  + exfalso.
+    apply Permutation_Type_vs_elt_inv in HP.
+    specialize (Hgax a).
+    destruct HP as [[l1 l2] Heq] ; rewrite Heq in Hgax.
+    apply Forall_elt in Hgax.
+    inversion Hgax.
+  + exfalso.
+    apply Permutation_Type_vs_elt_inv in HP.
+    specialize (Hgax a).
+    destruct HP as [[l1 l2] Heq] ; rewrite Heq in Hgax.
+    apply Forall_elt in Hgax.
+    inversion Hgax.
+  + exfalso.
+    apply Permutation_Type_vs_elt_inv in HP.
+    specialize (Hgax a).
+    destruct HP as [[l1 l2] Heq] ; rewrite Heq in Hgax.
+    apply Forall_elt in Hgax.
+    inversion Hgax.
+Qed.
 
 Lemma ll_to_mix2_cut {P} : forall l,
   ll P (wn (tens bot bot) :: l) -> ll (mk_pfrag true P.(pgax) P.(pmix0) true P.(pperm)) l.
@@ -377,6 +1191,31 @@ Qed.
 
 (** Provability in [ll_mix02] is equivalent to adding [wn (tens (wn one) (wn one))] in [ll] *)
 
+Lemma mix02_to_ll {P} : pperm P = true -> forall b1 b2 bp l,
+  ll (mk_pfrag P.(pcut) P.(pgax) b1 b2 bp) l -> ll P (wn (tens (wn one) (wn one)) :: l).
+Proof with myeeasy ; try PCperm_Type_solve.
+intros fp b1 b2 bp l pi.
+eapply (ext_wn_param _ P fp _ (tens (wn one) (wn one) :: nil)) in pi.
+- eapply ex_r...
+- intros Hcut...
+- simpl ; intros a.
+  eapply ex_r ; [ | apply PCperm_Type_last ].
+  apply wk_r.
+  apply gax_r.
+- intros Hpmix0 Hpmix0'.
+  apply de_r...
+  rewrite <- (app_nil_l nil).
+  apply tens_r ; apply de_r ; apply one_r.
+- intros _ _ l1 l2 pi1 pi2.
+  apply (ex_r _ (wn (tens (wn one) (wn one)) :: l2 ++ l1))...
+  apply co_r.
+  apply co_r.
+  apply de_r.
+  eapply ex_r.
+  + apply tens_r ; apply wk_r ; [ apply pi1 | apply pi2 ].
+  + rewrite fp...
+Qed.
+
 Lemma ll_to_mix02_cut {P} : forall l,
   ll P (wn (tens (wn one) (wn one)) :: l) -> ll (mk_pfrag true P.(pgax) true true P.(pperm)) l.
 Proof with myeasy.
@@ -402,6 +1241,125 @@ eapply stronger_pfrag in pi.
   + destruct pmix0...
   + destruct pmix2...
 Qed.
+
+(** Provability in [ll_mix02] is equivalent to adding other stuff in [ll] *)
+
+Lemma mix02_to_ll' {P} : pperm P = true -> forall b0 b2 bp l,
+  ll (mk_pfrag P.(pcut) P.(pgax) b0 b2 bp) l -> ll P (wn one :: wn (tens bot bot) :: l).
+Proof with myeasy.
+intros Hperm b0 b2 bp l pi.
+eapply mix0_to_ll...
+eapply mix2_to_ll...
+apply pi.
+Qed.
+
+Lemma ll_to_mix02'_axat {P} : (forall a, Forall atomic (projT2 (pgax P) a)) ->
+  pperm P = true -> forall l,
+  ll P (wn one :: wn (tens bot bot) :: l) -> ll (mix2add_pfrag (mix0add_pfrag P)) l.
+Proof with myeasy.
+intros Hgax Hperm l pi.
+apply ll_to_mix2_axat...
+apply ll_to_mix0_axat...
+Qed.
+
+Lemma mix02_to_ll'' {P} : pperm P = true -> forall b0 b2 bp l,
+  ll (mk_pfrag P.(pcut) P.(pgax) b0 b2 bp) l -> ll P (wn one :: wn (tens (wn one) bot) :: l).
+Proof with myeeasy ; try PCperm_Type_solve.
+intros Hperm b0 b2 bp l pi.
+eapply (ext_wn_param _ _ _ _ (one :: tens (wn one) bot :: nil)) in pi.
+- eapply ex_r...
+- intros Hcut...
+- simpl ; intros a.
+  eapply ex_r ; [ | apply PCperm_Type_app_comm ] ; list_simpl.
+  apply wk_r.
+  apply wk_r.
+  apply gax_r.
+- intros Hpmix0 Hpmix0'.
+  apply de_r...
+  eapply ex_r ; [ | apply PCperm_Type_swap ].
+  apply wk_r.
+  apply one_r.
+- intros _ _ l1 l2 pi1 pi2.
+  apply (ex_r _ (wn (tens (wn one) bot) :: (wn one :: l2) ++ l1)) ; [ | rewrite Hperm ]...
+  apply co_r.
+  apply co_r.
+  apply de_r.
+  apply (ex_r _ (tens (wn one) bot :: (wn (tens (wn one) bot) :: wn one :: l2)
+                                   ++ (wn (tens (wn one) bot) :: l1))) ;
+    [ | rewrite Hperm ]...
+  apply tens_r.
+  + eapply ex_r ; [ apply pi1 | ]...
+  + apply bot_r ; eapply ex_r ; [ apply pi2 | rewrite Hperm ]...
+Unshelve. assumption.
+Qed.
+
+(* Hgax_cut is here only to allow the use of cut_admissible
+   the more general result without Hgax_cut should be provable by induction as for [ll_to_mix2] *)
+Lemma ll_to_mix02''_axcut {P} : (forall a, Forall atomic (projT2 (pgax P) a)) ->
+  (forall a b x l1 l2 l3 l4,
+     projT2 (pgax P) a = (l1 ++ dual x :: l2) -> projT2 (pgax P) b = (l3 ++ x :: l4) ->
+     { c | projT2 (pgax P) c = l3 ++ l2 ++ l1 ++ l4 }) ->
+  pperm P = true -> forall l,
+  ll P (wn one :: wn (tens (wn one) bot) :: l) -> ll (mix2add_pfrag (mix0add_pfrag P)) l.
+Proof with myeasy.
+intros Hgax_at Hgax_cut Hperm l pi.
+apply (stronger_pfrag (cutrm_pfrag (cutupd_pfrag (mix2add_pfrag (mix0add_pfrag P)) true))).
+{ nsplit 5...
+  intros a ; exists a... }
+eapply cut_admissible...
+eapply stronger_pfrag in pi.
+- rewrite <- (app_nil_r l).
+  eapply (cut_r _ (wn (tens (wn one) bot))) ; simpl.
+  + change nil with (map wn nil).
+    apply oc_r.
+    apply parr_r.
+    change (one :: oc bot :: map wn nil) with ((one :: nil) ++ oc bot :: map wn nil).
+    eapply mix2_r...
+    * apply oc_r.
+      apply bot_r.
+      apply mix0_r...
+    * apply one_r.
+  + rewrite <- app_nil_r.
+    eapply cut_r ; [ | | apply pi ] ; simpl...
+    change nil with (map wn nil).
+    apply oc_r.
+    apply bot_r.
+    apply mix0_r...
+- etransitivity ; [ apply cutupd_pfrag_true| ].
+  nsplit 5...
+  + intros a ; exists a...
+  + apply leb_true.
+  + apply leb_true.
+Unshelve. reflexivity.
+Qed.
+
+(* Hgax_cut is here only to allow the use of cut_admissible
+   the more general result without Hgax_cut should be provable by induction as for [ll_to_mix2] *)
+Lemma ll_to_mix02'''_axcut {P} : (forall a, Forall atomic (projT2 (pgax P) a)) ->
+  (forall a b x l1 l2 l3 l4,
+     projT2 (pgax P) a = (l1 ++ dual x :: l2) -> projT2 (pgax P) b = (l3 ++ x :: l4) ->
+     { c | projT2 (pgax P) c = l3 ++ l2 ++ l1 ++ l4 }) ->
+  pperm P = true -> forall l (l0 : list unit),
+  ll P (wn one :: map (fun _ => wn (tens (wn one) bot)) l0 ++ l)  ->
+  ll (mix2add_pfrag (mix0add_pfrag P)) l.
+Proof with try assumption.
+intros Hgax_at Hgax_cut Hperm l l0 pi.
+apply ll_to_mix02''_axcut...
+revert l pi ; induction l0 ; intros l pi.
+- cons2app.
+  eapply ex_r ; [ | rewrite Hperm ; apply Permutation_Type_app_comm ].
+  simpl ; apply wk_r.
+  eapply ex_r ; [ | rewrite Hperm ; apply Permutation_Type_app_comm ]...
+- cons2app.
+  eapply ex_r ; [ | rewrite Hperm ; apply Permutation_Type_app_comm ].
+  simpl ; apply co_r.
+  rewrite 2 app_comm_cons.
+  eapply ex_r ; [ | rewrite Hperm ; apply Permutation_Type_app_comm ].
+  list_simpl ; apply IHl0.
+  list_simpl in pi.
+  eapply ex_r ; [ apply pi | rewrite Hperm ; PCperm_Type_solve ].
+Qed.
+
 
 (** Provability in [ll_mix02] is equivalent to provability of [ll]
 extended with the provability of both [bot :: bot :: nil] and [one :: one :: nil] *)
